Risc0/MlirTactics.lean
@@ -103,7 +103,9 @@ elab "MLIR" : tactic => do
   evalTactic <| ← `(
     tactic| repeat MLIR_statement
   )
-  evalTactic <| ← `(tactic| try simp? [Buffer.back_def.symm, isGetValid_def.symm, getImpl_def.symm, -zero_le, -zero_le', -Nat.zero_le])
+  evalTactic <| ← `(tactic| try simp? [
+    Buffer.back_def.symm, isGetValid_def.symm, getImpl_def.symm, addImpl_def.symm,
+    iszImpl_def.symm, invImpl_def.symm, -zero_le, -zero_le', -Nat.zero_le])
   
 -- elab "MLIR_statement" : tactic => do
 --   evalTactic <| ← `(
